src/Mail2/MailboxAPI.v
@@ -1,6 +1,4 @@
 Require Import POCS.
-Require Import FMapInterface.
-Require Import FMapAVL.
 Require Import String.
 Require Import MailServerAPI.
 Require Import MailServerDirAPI.
