src/Mail2/MailboxTmpAbsAPI.v
@@ -1,0 +1,60 @@
+Require Import POCS.
+Require Import String.
+Require Import MailboxAPI.
+Require Import MailServerDirAPI.
+
+
+Module MailboxTmpAbsAPI <: Layer.
+
+  Import MailboxAPI.
+  Import MailServerDirAPI.
+
+  Definition opT := xopT.
+
+  Record state_rec := mk_state {
+    tmpdir : dir_contents;
+    maildir : dir_contents;
+  }.
+
+  Definition State := state_rec.
+  Definition initP (s : State) := True.
+
+  Inductive xstep : forall T, opT T -> nat -> State -> T -> State -> list event -> Prop :=
+  | StepDeliver : forall m tmp mbox tid fn,
+    ~ FMap.In fn mbox ->
+    xstep (Deliver m) tid
+      (mk_state tmp mbox)
+      tt
+      (mk_state tmp (FMap.add fn m mbox))
+      nil
+  | StepList : forall tmp mbox tid r,
+    FMap.is_permutation_key r mbox ->
+    xstep List tid
+      (mk_state tmp mbox)
+      r
+      (mk_state tmp mbox)
+      nil
+  | StepRead : forall fn tmp mbox tid m,
+    FMap.MapsTo fn m mbox ->
+    xstep (Read fn) tid
+      (mk_state tmp mbox)
+      m
+      (mk_state tmp mbox)
+      nil
+  | StepGetRequest : forall s tid r,
+    xstep GetRequest tid
+      s
+      r
+      s
+      (Event r :: nil)
+  | StepRespond : forall s tid T (v : T),
+    xstep (Respond v) tid
+      s
+      tt
+      s
+      (Event v :: nil)
+  .
+
+  Definition step := xstep.
+
+End MailboxTmpAbsAPI.
