src/Mail2/MailboxTmpAbsImpl.v
@@ -1,0 +1,57 @@
+Require Import POCS.
+Require Import MailboxAPI.
+Require Import MailboxTmpAbsAPI.
+
+
+Module MailboxTmpAbs <: LayerImpl MailboxTmpAbsAPI MailboxAPI.
+
+  Definition absR (s1 : MailboxTmpAbsAPI.State) (s2 : MailboxAPI.State) :=
+    MailboxTmpAbsAPI.maildir s1 = s2.
+
+  Definition compile_ts (ts : @threads_state MailboxAPI.opT) := ts.
+
+  Theorem compile_ts_no_atomics :
+    forall (ts : @threads_state MailboxAPI.opT),
+      no_atomics_ts ts ->
+      no_atomics_ts (compile_ts ts).
+  Proof.
+    unfold compile_ts; eauto.
+  Qed.
+
+  Hint Extern 1 (MailboxAPI.step _ _ _ _ _ _) => econstructor.
+
+  Theorem absR_ok :
+    op_abs absR MailboxTmpAbsAPI.step MailboxAPI.step.
+  Proof.
+    unfold op_abs, absR; intros.
+    destruct s1; simpl in *; subst.
+    inversion H0; clear H0; subst; repeat sigT_eq.
+    all: eauto 10.
+  Qed.
+
+  Hint Resolve absR_ok.
+
+  Theorem compile_traces_match :
+    forall ts,
+      no_atomics_ts ts ->
+      traces_match_abs absR
+        MailboxTmpAbsAPI.initP
+        MailboxTmpAbsAPI.step
+        MailboxAPI.step (compile_ts ts) ts.
+  Proof.
+    unfold compile_ts, traces_match_abs; intros.
+    eexists; intuition idtac.
+    eapply trace_incl_abs; eauto.
+    eauto.
+  Qed.
+
+  Theorem absInitP :
+    forall s1 s2,
+      MailboxTmpAbsAPI.initP s1 ->
+      absR s1 s2 ->
+      MailboxAPI.initP s2.
+  Proof.
+    eauto.
+  Qed.
+
+End MailboxTmpAbs.
